Checks/Bls12381G1AddSourceFiniteUnequal.lean
@@ -155,4 +155,10 @@ example (yst : EvmState)
 #guard_msgs in
 #print axioms mainFiniteUnequalDenominatorArgsState_loadWord
 
+/-- info: 'Challenge.Bls12381G1Add.Reference.Proofs.SourceSemantics.eval_fpSubLoads' depends on axioms: [propext,
+ Classical.choice,
+ Quot.sound] -/
+#guard_msgs in
+#print axioms eval_fpSubLoads
+
 end Challenge.Bls12381G1Add.Reference.Proofs.SourceSemantics
